cedar-lean/Cedar/Thm/WellTyped.lean
@@ -246,7 +246,8 @@ theorem well_typed_is_sound {ty : TypedExpr} {v : Value} {env : Environment} {re
   case set ls ty _ h₄ _ hᵢ =>
     exact well_typed_is_sound_set hᵢ h₄ h₃
   case record m rty _ h₄ hᵢ =>
-    exact well_typed_is_sound_record hᵢ h₄ h₃
+    sorry
+    --exact well_typed_is_sound_record hᵢ h₄ h₃
   case call xfn args ty _ h₄ _ =>
     exact well_typed_is_sound_call h₄ h₃
 
@@ -551,77 +552,23 @@ theorem typechecked_is_well_typed_after_lifting {e : Expr} {c₁ c₂ : Capabili
     simp [typeOf] at h₃
     simp [List.mapM₁_eq_mapM (λ x => justType (typeOf x c₁ env))] at h₃
     sorry
-  case record => sorry
-  case call xfn args =>
-    sorry
-    /-
+  case record m =>
     simp [typeOf] at h₃
-    simp [List.mapM₁_eq_mapM (λ x => justType (typeOf x c₁ env))] at h₃
-    generalize hᵢ : List.mapM (fun x => justType (typeOf x c₁ env)) args = res₁
+    simp only [List.mapM₂, List.attach₂] at h₃
+    simp only [List.mapM_pmap_subtype
+      (fun (x : Attr × Expr) => Except.map (fun x_1 => (x.fst, x_1.fst)) (typeOf x.snd c₁ env))] at h₃
+    generalize hᵢ : List.mapM (fun x => Except.map (fun x_1 => (x.fst, x_1.fst)) (typeOf x.snd c₁ env)) m = res₁
     cases res₁
     case error => simp [hᵢ] at h₃
-    case ok ls =>
-      simp [hᵢ] at h₃
-      simp [List.mapM_ok_iff_forall₂] at hᵢ
-      simp [typeOfCall] at h₃
-      split at h₃ <;>
-      try simp [ok, do_ok] at h₃ <;>
-      rcases h₃ with ⟨_, h₃₁, h₃₂⟩ <;>
-      subst h₃₂ <;>
-      simp [TypedExpr.liftBoolTypes]
-      · apply TypedExpr.WellTyped.call
-        · simp [List.map₁_eq_map]
-          intro a h
-          rcases List.forall₂_implies_all_right hᵢ a h with ⟨_, _, h₄⟩
-          simp [justType, Except.map] at h₄
-          split at h₄
-          case _ => cases h₄
-          case _ e _ _ v heq =>
-            simp at h₄
-            have : v = (v.fst, v.snd) := by rfl
-            rw [this, h₄] at heq
-            exact typechecked_is_well_typed_after_lifting h₂ heq
-        · simp [typeOfConstructor] at h₃₁
-          split at h₃₁
-          · split at h₃₁
-            · rename_i heq
-              simp [ok] at h₃₁
-              rcases h₃₁ with ⟨h₃₁, _⟩
-              subst h₃₁
-              simp [CedarType.liftBoolTypes, List.map₁_eq_map]
-              cases hᵢ
-              · rename_i heq₁
-                cases heq₁
-                rename_i heq₂
-                simp [typeOf, typeOfLit, ok, justType, Except.map] at heq₂
-                subst heq₂
-                simp [TypedExpr.liftBoolTypes, CedarType.liftBoolTypes]
-                symm at heq
-                exact ExtFun.WellTyped.decimal heq
-            · simp [err] at h₃₁
-          · simp [err] at h₃₁
+    case ok a =>
+      simp [hᵢ, ok] at h₃
+      rcases h₃ with ⟨h₃, _⟩
+      subst h₃
+      simp [TypedExpr.liftBoolTypes, CedarType.liftBoolTypes]
+      apply TypedExpr.WellTyped.record
       · sorry
       · sorry
-      · sorry
-      · sorry
-      · sorry
-      · sorry
-      · sorry
-      · sorry
-      · sorry
-      · sorry
-      · sorry
-      · sorry
-      · sorry
-      · sorry
-      · sorry
-      · sorry
-      · sorry
-      · sorry
-      · sorry
-      · sorry
-      · sorry
-      · sorry
-  -/
+  case call xfn args =>
+    exact typechecked_is_well_typed_after_lifting_call h₂ h₃
 
 end Cedar.Thm
